extracted/sld_interpreter_wrapped.hs
@@ -208,14 +208,8 @@ unification_step t1 t2 =
          x -> x};
        Right -> NonUnifiable}}}
 
-data Mgu =
-   MguNonUnifiable Term Term
- | MguSame Term Term
- | MguVarSubstNone Term Term Name Term Mgu
- | MguVarSubstSome Term Term Name Term Subst Subst Mgu
-
-mgu_exists :: Term -> Term -> SigT (Option Subst) Mgu
-mgu_exists t1 t2 =
+mgu_result_exists :: Term -> Term -> SigT (Option Subst) ()
+mgu_result_exists t1 t2 =
   let {
    h = well_founded_induction (\x h ->
          eq_rec_r __ (\h0 ->
@@ -223,8 +217,8 @@ mgu_exists t1 t2 =
             Pair t3 t4 ->
              let {u = unification_step t3 t4} in
              case u of {
-              NonUnifiable -> ExistT None (MguNonUnifiable t3 t4);
-              Same -> ExistT (Some empty_subst) (MguSame t3 t4);
+              NonUnifiable -> ExistT None __;
+              Same -> ExistT (Some empty_subst) __;
               VarSubst n t ->
                let {
                 h1 = h0 (Pair (apply_subst (singleton_subst n t) t3)
@@ -232,15 +226,17 @@ mgu_exists t1 t2 =
                in
                let {h2 = h1 __} in
                case h2 of {
-                ExistT x0 m ->
+                ExistT x0 _ ->
                  case x0 of {
                   Some s -> ExistT (Some (compose (singleton_subst n t) s))
-                   (MguVarSubstSome t3 t4 n t s
-                   (compose (singleton_subst n t) s) m);
-                  None -> ExistT None (MguVarSubstNone t3 t4 n t m)}}}}) __ h)
-         (Pair t1 t2)}
+                   __;
+                  None -> ExistT None __}}}}) __ h) (Pair t1 t2)}
   in
   eq_rec_r __ (\h0 -> h0) __ h
+
+data Stream a =
+   Nil0
+ | Cons0 a (Stream a)
 
 data Goal =
    Fail
@@ -257,42 +253,34 @@ type Def = Rel
 
 type Spec = Name -> Def
 
-data Stream a =
-   Nil0
- | Cons0 a (Stream a)
-
-helper :: (Stream a1) -> Stream a1
-helper s =
-  s
-
 data Cutting_mark =
    StopCutting
  | KeepCutting
 
-data State' =
+data Nt_state =
    Leaf Goal Subst Nat
- | Sum Cutting_mark State' State'
- | Prod0 State' Goal
+ | Sum Cutting_mark Nt_state Nt_state
+ | Prod0 Nt_state Goal
 
-state'_rect :: (Goal -> Subst -> Nat -> a1) -> (Cutting_mark -> State' -> a1
-               -> State' -> a1 -> a1) -> (State' -> a1 -> Goal -> a1) ->
-               State' -> a1
-state'_rect f f0 f1 s =
-  case s of {
-   Leaf g s0 n -> f g s0 n;
-   Sum c s0 s1 ->
-    f0 c s0 (state'_rect f f0 f1 s0) s1 (state'_rect f f0 f1 s1);
-   Prod0 s0 g -> f1 s0 (state'_rect f f0 f1 s0) g}
+nt_state_rect :: (Goal -> Subst -> Nat -> a1) -> (Cutting_mark -> Nt_state ->
+                 a1 -> Nt_state -> a1 -> a1) -> (Nt_state -> a1 -> Goal ->
+                 a1) -> Nt_state -> a1
+nt_state_rect f f0 f1 n =
+  case n of {
+   Leaf g s n0 -> f g s n0;
+   Sum c n0 n1 ->
+    f0 c n0 (nt_state_rect f f0 f1 n0) n1 (nt_state_rect f f0 f1 n1);
+   Prod0 n0 g -> f1 n0 (nt_state_rect f f0 f1 n0) g}
 
-state'_rec :: (Goal -> Subst -> Nat -> a1) -> (Cutting_mark -> State' -> a1
-              -> State' -> a1 -> a1) -> (State' -> a1 -> Goal -> a1) ->
-              State' -> a1
-state'_rec =
-  state'_rect
+nt_state_rec :: (Goal -> Subst -> Nat -> a1) -> (Cutting_mark -> Nt_state ->
+                a1 -> Nt_state -> a1 -> a1) -> (Nt_state -> a1 -> Goal -> a1)
+                -> Nt_state -> a1
+nt_state_rec =
+  nt_state_rect
 
-data State0 =
+data State =
    Stop
- | State State'
+ | NTState Nt_state
 
 data Label =
    Step
@@ -302,135 +290,91 @@ data Cut_signal =
    NoCutting
  | YesCutting
 
-data Eval_step_SLD =
-   EsFail Subst Nat
- | EsCut Subst Nat
- | EsUnifyFail Term Term Subst Nat Mgu
- | EsUnifySuccess Term Term Subst Subst Nat Mgu
- | EsDisj Goal Goal Subst Nat
- | EsConj Goal Goal Subst Nat
- | EsFresh (Name -> Goal) Subst Nat
- | EsInvoke Name Term Subst Nat
- | EsSumE State' Cutting_mark State' Label Eval_step_SLD
- | EsSumECS State' State' Label Eval_step_SLD
- | EsSumECK State' State' Label Eval_step_SLD
- | EsSumNE State' Cutting_mark State' State' Label Eval_step_SLD
- | EsSumNEC State' State' State' Label Eval_step_SLD
- | EsSumNEK State' State' State' Label Eval_step_SLD
- | EsProdSE State' Goal Cut_signal Eval_step_SLD
- | EsProdAE State' Goal Subst Nat Cut_signal Eval_step_SLD
- | EsProdSNE State' Goal Cut_signal State' Eval_step_SLD
- | EsProdANE State' Goal Subst Nat Cut_signal State' Eval_step_SLD
-
-eval_step_SLD_exists :: State' -> SigT Label
-                        (SigT Cut_signal (SigT State0 Eval_step_SLD))
-eval_step_SLD_exists st' =
-  state'_rec (\g s n ->
+eval_step_exists :: Nt_state -> SigT Label (SigT Cut_signal (SigT State ()))
+eval_step_exists nst =
+  nt_state_rec (\g s n ->
     case g of {
-     Fail -> ExistT Step (ExistT NoCutting (ExistT Stop (EsFail s n)));
-     Cut -> ExistT (Answer s n) (ExistT YesCutting (ExistT Stop (EsCut s n)));
+     Fail -> ExistT Step (ExistT NoCutting (ExistT Stop __));
+     Cut -> ExistT (Answer s n) (ExistT YesCutting (ExistT Stop __));
      Unify t t0 ->
-      let {h = mgu_exists (apply_subst s t) (apply_subst s t0)} in
+      let {h = mgu_result_exists (apply_subst s t) (apply_subst s t0)} in
       case h of {
-       ExistT x m ->
+       ExistT x _ ->
         case x of {
          Some s0 -> ExistT (Answer (compose s s0) n) (ExistT NoCutting
-          (ExistT Stop (EsUnifySuccess t t0 s s0 n m)));
-         None -> ExistT Step (ExistT NoCutting (ExistT Stop (EsUnifyFail t t0
-          s n m)))}};
-     Disj g1 g2 -> ExistT Step (ExistT NoCutting (ExistT (State (Sum
-      StopCutting (Leaf g1 s n) (Leaf g2 s n))) (EsDisj g1 g2 s n)));
-     Conj g1 g2 -> ExistT Step (ExistT NoCutting (ExistT (State (Prod0 (Leaf
-      g1 s n) g2)) (EsConj g1 g2 s n)));
-     Fresh g0 -> ExistT Step (ExistT NoCutting (ExistT (State (Leaf (g0 n) s
-      (S n))) (EsFresh g0 s n)));
-     Invoke n0 t -> ExistT Step (ExistT NoCutting (ExistT (State (Leaf
-      (proj1_sig (prog n0) t) s n)) (EsInvoke n0 t s n)))})
-    (\c st'1 iHst'1 st'2 _ ->
-    case iHst'1 of {
+          (ExistT Stop __));
+         None -> ExistT Step (ExistT NoCutting (ExistT Stop __))}};
+     Disj g1 g2 -> ExistT Step (ExistT NoCutting (ExistT (NTState (Sum
+      StopCutting (Leaf g1 s n) (Leaf g2 s n))) __));
+     Conj g1 g2 -> ExistT Step (ExistT NoCutting (ExistT (NTState (Prod0
+      (Leaf g1 s n) g2)) __));
+     Fresh g0 -> ExistT Step (ExistT NoCutting (ExistT (NTState (Leaf 
+      (g0 n) s (S n))) __));
+     Invoke n0 t -> ExistT Step (ExistT NoCutting (ExistT (NTState (Leaf
+      (proj1_sig (prog n0) t) s n)) __))}) (\c _ iHnst1 nst2 _ ->
+    case iHnst1 of {
      ExistT l1 s ->
       case s of {
        ExistT cs s0 ->
         case s0 of {
-         ExistT st1 iH1 ->
+         ExistT st1 _ ->
           case st1 of {
            Stop ->
             case cs of {
-             NoCutting -> ExistT l1 (ExistT NoCutting (ExistT (State st'2)
-              (EsSumE st'1 c st'2 l1 iH1)));
+             NoCutting -> ExistT l1 (ExistT NoCutting (ExistT (NTState nst2)
+              __));
              YesCutting ->
               case c of {
-               StopCutting -> ExistT l1 (ExistT NoCutting (ExistT Stop
-                (EsSumECS st'1 st'2 l1 iH1)));
-               KeepCutting -> ExistT l1 (ExistT YesCutting (ExistT Stop
-                (EsSumECK st'1 st'2 l1 iH1)))}};
-           State s1 ->
+               StopCutting -> ExistT l1 (ExistT NoCutting (ExistT Stop __));
+               KeepCutting -> ExistT l1 (ExistT YesCutting (ExistT Stop __))}};
+           NTState n ->
             case cs of {
-             NoCutting -> ExistT l1 (ExistT NoCutting (ExistT (State (Sum c
-              s1 st'2)) (EsSumNE st'1 c s1 st'2 l1 iH1)));
+             NoCutting -> ExistT l1 (ExistT NoCutting (ExistT (NTState (Sum c
+              n nst2)) __));
              YesCutting ->
               case c of {
-               StopCutting -> ExistT l1 (ExistT NoCutting (ExistT (State s1)
-                (EsSumNEC st'1 s1 st'2 l1 iH1)));
-               KeepCutting -> ExistT l1 (ExistT YesCutting (ExistT (State s1)
-                (EsSumNEK st'1 s1 st'2 l1 iH1)))}}}}}}) (\st'0 iHst' g ->
-    case iHst' of {
+               StopCutting -> ExistT l1 (ExistT NoCutting (ExistT (NTState n)
+                __));
+               KeepCutting -> ExistT l1 (ExistT YesCutting (ExistT (NTState
+                n) __))}}}}}}) (\_ iHnst g ->
+    case iHnst of {
      ExistT l s ->
       case s of {
        ExistT cs s0 ->
         case s0 of {
-         ExistT st iH ->
+         ExistT st _ ->
           case st of {
            Stop ->
             case l of {
-             Step -> ExistT Step (ExistT cs (ExistT Stop (EsProdSE st'0 g cs
-              iH)));
-             Answer s1 n -> ExistT Step (ExistT cs (ExistT (State (Leaf g s1
-              n)) (EsProdAE st'0 g s1 n cs iH)))};
-           State s1 ->
+             Step -> ExistT Step (ExistT cs (ExistT Stop __));
+             Answer s1 n -> ExistT Step (ExistT cs (ExistT (NTState (Leaf g
+              s1 n)) __))};
+           NTState n ->
             case l of {
-             Step -> ExistT Step (ExistT cs (ExistT (State (Prod0 s1 g))
-              (EsProdSNE st'0 g cs s1 iH)));
-             Answer s2 n -> ExistT Step (ExistT cs (ExistT (State (Sum
-              KeepCutting (Leaf g s2 n) (Prod0 s1 g))) (EsProdANE st'0 g s2 n
-              cs s1 iH)))}}}}}) st'
+             Step -> ExistT Step (ExistT cs (ExistT (NTState (Prod0 n g))
+              __));
+             Answer s1 n0 -> ExistT Step (ExistT cs (ExistT (NTState (Sum
+              KeepCutting (Leaf g s1 n0) (Prod0 n g))) __))}}}}}) nst
 
 type Trace = Stream Label
 
-data Op_sem_SLD =
-   OsStop
- | OsState State' Label Cut_signal State0 Trace Eval_step_SLD Op_sem_SLD
-
-trace_from :: State0 -> Trace
+trace_from :: State -> Trace
 trace_from st =
   case st of {
    Stop -> Nil0;
-   State st' ->
-    case eval_step_SLD_exists st' of {
+   NTState nst ->
+    case eval_step_exists nst of {
      ExistT l s ->
       case s of {
        ExistT _ s0 ->
         case s0 of {
-         ExistT st'' _ -> Cons0 l (trace_from st'')}}}}
+         ExistT nst' _ -> Cons0 l (trace_from nst')}}}}
 
-trace_from_correct :: State0 -> Op_sem_SLD
-trace_from_correct st =
-  case st of {
-   Stop -> eq_rec_r (helper (trace_from Stop)) OsStop (trace_from Stop);
-   State s ->
-    eq_rec_r (helper (trace_from (State s)))
-      (let {s0 = eval_step_SLD_exists s} in
-       case s0 of {
-        ExistT l s1 ->
-         case s1 of {
-          ExistT cs s2 ->
-           case s2 of {
-            ExistT st0 eV -> OsState s l cs st0 (trace_from st0) eV
-             (trace_from_correct st0)}}}) (trace_from (State s))}
+op_sem_exists :: State -> SigT Trace ()
+op_sem_exists st =
+  ExistT (trace_from st) __
 
-op_sem_SLD_exists :: State0 -> SigT Trace Op_sem_SLD
-op_sem_SLD_exists st =
-  ExistT (trace_from st) (trace_from_correct st)
+
 
 
 
@@ -685,11 +629,11 @@ streamToList :: Stream a -> [a]
 streamToList Nil0         = []
 streamToList (Cons0 x xs) = x : streamToList xs
 
-initState :: P.Int -> Atom -> State0
-initState n a = State (Leaf (translate_atom a) Nil (int_to_nat n))
+initState :: P.Int -> Atom -> State
+initState n a = NTState (Leaf (translate_atom a) Nil (int_to_nat n))
 
 interpret :: P.Int -> Atom -> [Subst]
-interpret n a = let (ExistT t _) = op_sem_SLD_exists (initState n a)
+interpret n a = let (ExistT t _) = op_sem_exists (initState n a)
                 in P.map (\ (Answer s _) ->  s) (P.filter answersOnly (streamToList t))
   where
     answersOnly Step = P.False
