src/InterleavingSearch/Soundness.v
@@ -2,64 +2,77 @@ Require Import List.
 Require Import Coq.Lists.ListSet.
 Import ListNotations.
 Require Import Omega.
-Require Import Coq.Program.Equality.
 
-Require Import Stream.
-Require Import Unify.
-Require Import MiniKanrenSyntaxDiseq.
-Require Import DenotationalSemDiseq.
-Require Import OperationalSemDiseq.
+Require Import Unification.
+Require Import Streams.
+Require Import Language.
+Require Import DenotationalSem.
+Require Import OperationalSem.
+
+Inductive in_denotational_sem_nt_state : nt_state -> repr_fun -> Prop :=
+| dsnstLeaf : forall g s n f (DSG  : [| g , f |])
+                             (DSS  : [ s , f ]),
+                             in_denotational_sem_nt_state (Leaf g s n) f
+| dsnstSumL : forall nst1 nst2 f (DSST' : in_denotational_sem_nt_state nst1 f),
+                                 in_denotational_sem_nt_state (Sum nst1 nst2) f
+| dsnstSumR : forall nst1 nst2 f (DSST' : in_denotational_sem_nt_state nst2 f),
+                                 in_denotational_sem_nt_state (Sum nst1 nst2) f
+| dsnstProd : forall nst g f (DSG : [| g , f |])
+                             (DSST' : in_denotational_sem_nt_state nst f),
+                             in_denotational_sem_nt_state (Prod nst g) f.
+
+Hint Constructors in_denotational_sem_nt_state : core.
+
+Inductive in_denotational_sem_state : state -> repr_fun -> Prop :=
+| dsstNTState : forall nst f (DSST' : in_denotational_sem_nt_state nst f),
+                           in_denotational_sem_state (NTState nst) f.
+
+Hint Constructors in_denotational_sem_state : core.
+
 
 Lemma answer_correct
       (s : subst)
-      (cs : constraint_store s)
       (n : nat)
       (f : repr_fun)
       (DSS : [ s , f ])
-      (DSCS : [| s , cs , f |])
-      (st' : state')
+      (st' : nt_state)
       (st : state)
-      (EV : eval_step st' (Answer s cs n) st) :
-      in_denotational_sem_state' st' f.
+      (EV : eval_step st' (Answer s n) st) :
+      in_denotational_sem_nt_state st' f.
 Proof.
-  remember (Answer s cs n) as l.
-  induction EV; good_inversion Heql; simpl_existT_cs_same; auto.
+  remember (Answer s n) as l.
+  induction EV; good_inversion Heql; auto.
   { assert (DSS_copy := DSS). apply (denotational_sem_uni _ _ _ _ MGU _) in DSS.
-    destruct DSS as [DSS EQ]. constructor; auto.
-    eapply proj1. apply (upd_cs_success_condition _ _ _ _ UPD_CS f). auto. }
-  { specialize (add_constraint_success_condition _ _ _ _ _ ADD_C f). intro ADD_C_COND.
-    specialize (conj DSCS DSS). intro CONJ. apply ADD_C_COND in CONJ.
-    destruct CONJ as [DSCS0 [_ GT_NEQ]].
-    constructor; auto. }
+    destruct DSS as [DSS EQ]. constructor; auto. }
 Qed.
 
 Lemma next_state_correct
       (f : repr_fun)
       (st : state)
       (DSS : in_denotational_sem_state st f)
-      (st' : state')
-      (WF : well_formed_state' st')
+      (st' : nt_state)
+      (WF : well_formed_nt_state st')
       (h : label)
       (EV : eval_step st' h st) :
-      in_denotational_sem_state' st' f.
+      in_denotational_sem_nt_state st' f.
 Proof.
   induction EV; good_inversion DSS.
-  { good_inversion DSST'; good_inversion DSST'0; simpl_existT_cs_same;
+  { good_inversion DSST'; good_inversion DSST'0;
     constructor; auto. }
-  { good_inversion DSST'. good_inversion DSST'0. simpl_existT_cs_same. auto. }
-  { good_inversion WF. good_inversion DSST'. simpl_existT_cs_same.
+  { good_inversion DSST'. good_inversion DSST'0. auto. }
+  { good_inversion WF. good_inversion DSST'.
     constructor; auto. econstructor; eauto.
     intros HIn. apply FV_LT_COUNTER in HIn.
     { omega. }
     { reflexivity. } }
-  { good_inversion DSST'. simpl_existT_cs_same. auto. }
+  { good_inversion DSST'. auto. }
   { auto. }
   { good_inversion WF. good_inversion DSST'; auto. }
   { good_inversion DSST'. constructor; auto.
-    simpl_existT_cs_same. eapply answer_correct; eauto. }
+    eapply answer_correct; eauto. }
   { good_inversion WF. good_inversion DSST'. auto. }
   { good_inversion WF. good_inversion DSST'.
-    { good_inversion DSST'0. simpl_existT_cs_same.
+    { good_inversion DSST'0.
       constructor; auto.
       eapply answer_correct; eauto. }
     { good_inversion DSST'0. auto. } }
@@ -75,8 +88,8 @@ Lemma search_correctness_generalized
       in_denotational_sem_state st f.
 Proof.
   revert HOP WF. revert st.
-  red in HDA. destruct HDA as [s [cs [n [HInStr [DSS DSCS]]]]].
-  remember (Answer s cs n) as l. induction HInStr.
+  red in HDA. destruct HDA as [s [n [HInStr DSS]]].
+  remember (Answer s n) as l. induction HInStr.
   { intros. inversion HOP; clear HOP; subst.
     constructor. eapply answer_correct; eauto. }
   { specialize (IHHInStr Heql). intros.
@@ -88,33 +101,17 @@ Proof.
     constructor. eapply next_state_correct; eauto. }
 Qed.
 
-Fixpoint first_nats (k : nat) : list nat :=
-  match k with
-  | 0   => []
-  | S n => n :: first_nats n
-  end.
-
-Lemma first_nats_less
-      (n k : nat)
-      (H : In n (first_nats k)) :
-      n < k.
-Proof.
-  induction k.
-  { inversion H. }
-  { inversion H. { omega. } { apply IHk in H0. omega. } }
-Qed.
-
 Lemma search_correctness
       (g   : goal)
       (k   : nat)
       (HC  : closed_goal_in_context (first_nats k) g)
       (f   : repr_fun)
       (t   : trace)
-      (HOP : op_sem (State (Leaf g empty_subst init_cs k)) t)
+      (HOP : op_sem (NTState (Leaf g empty_subst k)) t)
       (HDA : {| t , f |}) :
       [| g , f |].
 Proof.
-  remember (State (Leaf g empty_subst init_cs k)) as st.
+  remember (NTState (Leaf g empty_subst k)) as st.
   assert (in_denotational_sem_state st f).
   { eapply search_correctness_generalized; eauto.
     subst. constructor. apply well_formed_initial_state; auto. }
