src/SLDSearch/LanguageSLD.v
@@ -3,19 +3,18 @@ Import ListNotations.
 Require Import Coq.Lists.ListSet.
 Require Import Arith.
 Require Import Omega.
-Require Import Unify.
+
+Require Import Unification.
 
 Inductive goal : Set :=
-| Fail     : goal
-| Cut      : goal                     (* for SLD semantics only, in others is treated as 'success' *)
-| Unify    : term -> term -> goal
-| Disunify : term -> term -> goal
-| Disj     : goal -> goal -> goal
-| Conj     : goal -> goal -> goal
-| Fresh    : (name -> goal) -> goal
-| Invoke   : name -> term -> goal.
+| Fail   : goal
+| Cut    : goal
+| Unify  : term -> term -> goal
+| Disj   : goal -> goal -> goal
+| Conj   : goal -> goal -> goal
+| Fresh  : (name -> goal) -> goal
+| Invoke : name -> term -> goal.
 
-(* rel is a body of a relational symbol *)
 Definition rel : Set := term -> goal.
 
 Inductive is_fv_of_goal (n : name) : goal -> Prop :=
@@ -23,10 +22,6 @@ Inductive is_fv_of_goal (n : name) : goal -> Prop :=
                           is_fv_of_goal n (Unify t1 t2)
 | fvUnifyR : forall t1 t2 (IN_FV : In n (fv_term t2)),
                           is_fv_of_goal n (Unify t1 t2)
-| fvDisunifyL : forall t1 t2 (IN_FV : In n (fv_term t1)),
-                             is_fv_of_goal n (Disunify t1 t2)
-| fvDisunifyR : forall t1 t2 (IN_FV : In n (fv_term t2)),
-                             is_fv_of_goal n (Disunify t1 t2)
 | fvDisjL  : forall g1 g2 (IS_FV : is_fv_of_goal n g1),
                           is_fv_of_goal n (Disj g1 g2)
 | fvDisjR  : forall g1 g2 (IS_FV : is_fv_of_goal n g2),
@@ -41,63 +36,9 @@ Inductive is_fv_of_goal (n : name) : goal -> Prop :=
 | fvInvoke : forall r arg (IN_FV : In n (fv_term arg)),
                           is_fv_of_goal n (Invoke r arg).
 
-Hint Constructors is_fv_of_goal.
+Hint Constructors is_fv_of_goal : core.
 
-Definition closed_goal_in_context (c : list name) (g : goal) : Prop :=
-  forall n, is_fv_of_goal n g -> In n c.
 
-Definition closed_goal : goal -> Prop := closed_goal_in_context [].
-
-Definition closed_rel (r : rel) : Prop :=
-  forall (arg : term), closed_goal_in_context (fv_term arg) (r arg).
-
-(* Some checks *)
-Module SmokeTest.
-
-  Definition g0 : goal := Fresh (fun x => Unify (Var x) (Cst 2)).
-  Definition g1 : goal := Fresh (fun x => Fresh (fun y => Unify (Var x) (Var y))).
-
-  Lemma g0_closed : closed_goal g0.
-  Proof.
-    red. red. intros. inversion H. inversion IS_FV.
-    { simpl in IN_FV. destruct IN_FV; contradiction. }
-    { inversion IN_FV. }
-  Qed.
-
-  Lemma g1_closed : closed_goal g1.
-  Proof.
-    red. red. intros. inversion H. inversion IS_FV.
-    inversion IS_FV0; inversion IN_FV; contradiction.
-  Qed.
-
-  Definition r0 : rel := (fun t => Fresh (fun x => Fresh (fun y =>
-      Conj (Unify t (Con 0 (Var x) (Var y))) (Unify (Var x) (Var y))))).
-  Definition r1 : rel := (fun t => Fresh (fun x => Unify (Var 0) t)).
-
-  Lemma r0_closed : closed_rel r0.
-  Proof.
-    red. red. intros. inversion H. inversion IS_FV.
-    inversion IS_FV0.
-    { inversion IS_FV; auto. inversion IS_FV2; inversion IS_FV3.
-      { auto. }
-      { simpl in IN_FV. destruct (name_eq_dec n'1 n').
-        { inversion IN_FV; contradiction. }
-        { inversion IN_FV; try contradiction. inversion H0; contradiction. } }
-      { inversion IN_FV; contradiction. }
-      { inversion IN_FV; contradiction. } }
-    { inversion IS_FV1; inversion IN_FV; contradiction. }
-  Qed.
-
-  Lemma r1_non_closed : ~ closed_rel r1.
-  Proof.
-    intro C. red in C. red in C.
-    specialize (C (Cst 0) 0). apply C.
-    unfold r1. apply fvFresh with 1.
-    { omega. }
-    { constructor. left. auto. }
-  Qed.
-
-End SmokeTest.
 
 (* Weak version of a variable renaming *)
 Inductive renaming (old_x : name) (new_x : name) : goal -> goal -> Prop :=
@@ -106,9 +47,6 @@ Inductive renaming (old_x : name) (new_x : name) : goal -> goal -> Prop :=
 | rUnify : forall t1 t2, renaming old_x new_x (Unify t1 t2)
                                               (Unify (apply_subst [(old_x, Var new_x)] t1)
                                                      (apply_subst [(old_x, Var new_x)] t2))
-| rDisunify : forall t1 t2, renaming old_x new_x (Disunify t1 t2)
-                                                 (Disunify (apply_subst [(old_x, Var new_x)] t1)
-                                                           (apply_subst [(old_x, Var new_x)] t2))
 | rDisj : forall g1 g2 rg1 rg2 (R_G1 : renaming old_x new_x g1 rg1)
                                (R_G2 : renaming old_x new_x g2 rg2),
                                renaming old_x new_x (Disj g1 g2) (Disj rg1 rg2)
@@ -124,7 +62,7 @@ Inductive renaming (old_x : name) (new_x : name) : goal -> goal -> Prop :=
 | rInvoke : forall r arg, renaming old_x new_x (Invoke r arg)
                                                (Invoke r (apply_subst [(old_x, Var new_x)] arg)).
 
-Hint Constructors renaming.
+Hint Constructors renaming : core.
 
 Definition consistent_binding (b : name -> goal) : Prop :=
   forall x y, (~ is_fv_of_goal x (Fresh b)) -> renaming x y (b x) (b y).
@@ -133,7 +71,6 @@ Inductive consistent_goal : goal -> Prop :=
 | cgFail   : consistent_goal Fail
 | cgCut    : consistent_goal Cut
 | cgUnify  : forall t1 t2, consistent_goal (Unify t1 t2)
-| cgDisunify  : forall t1 t2, consistent_goal (Disunify t1 t2)
 | cgDisj   : forall g1 g2 (CG_G1 : consistent_goal g1)
                           (CG_G2 : consistent_goal g2),
                           consistent_goal (Disj g1 g2)
@@ -145,7 +82,7 @@ Inductive consistent_goal : goal -> Prop :=
                        consistent_goal (Fresh fg)
 | cgInvoke : forall r arg, consistent_goal (Invoke r arg).
 
-Hint Constructors consistent_goal.
+Hint Constructors consistent_goal : core.
 
 Definition consistent_function (f : term -> goal) : Prop :=
   forall a1 a2 t, renaming a1 a2 (f t) (f (apply_subst [(a1, Var a2)] t)).
@@ -153,8 +90,18 @@ Definition consistent_function (f : term -> goal) : Prop :=
 Definition consistent_rel (r : rel) : Prop :=
   forall (arg : term), consistent_goal (r arg) /\ consistent_function r.
 
+
+
+Definition closed_goal_in_context (c : list name) (g : goal) : Prop :=
+  forall n, is_fv_of_goal n g -> In n c.
+
+Definition closed_rel (r : rel) : Prop :=
+  forall (arg : term), closed_goal_in_context (fv_term arg) (r arg).
+
+
+
 Definition def : Set := {r : rel | closed_rel r /\ consistent_rel r}.
 
 Definition spec : Set := name -> def.
 
-Variable Prog : spec.
+Axiom Prog : spec.
