src/InterleavingSearch/Completeness.v
@@ -1,0 +1,155 @@
+Require Import List.
+Require Import Coq.Lists.ListSet.
+Require Import Omega.
+
+Require Import Unification.
+Require Import Streams.
+Require Import Language.
+Require Import DenotationalSem.
+Require Import OperationalSem.
+
+
+Lemma search_completeness_generalized
+      (l    : nat)
+      (g    : goal)
+      (CG   : consistent_goal g)
+      (s    : subst)
+      (n    : nat)
+      (WF   : well_formed_nt_state (Leaf g s n))
+      (t    : trace)
+      (OP   : op_sem (NTState (Leaf g s n)) t)
+      (f    : repr_fun)
+      (DSG  : [| l | g , f |])
+      (DSS  : [ s , f ]) :
+      exists (f' : repr_fun), {| t , f' |} /\
+                            forall (x : name), x < n -> gt_eq (f x) (f' x).
+Proof.
+  revert OP. revert t. revert CG DSG DSS WF. revert g f s n. induction l.
+  { intros. apply in_denotational_sem_zero_lev in DSG. contradiction. }
+  { induction g; intros; good_inversion CG.
+    { good_inversion DSG. }
+    { exists f. split.
+      2: intros; red; auto.
+      good_inversion OP. good_inversion EV; good_inversion DSG.
+      { destruct DSS as [fs COMP_s_fs]. red in UNI.
+        rewrite <- (repr_fun_eq_apply _ _ t COMP_s_fs) in UNI.
+        rewrite <- (repr_fun_eq_apply _ _ t0 COMP_s_fs) in UNI.
+        rewrite (repr_fun_apply_compose s fs t) in UNI.
+        rewrite (repr_fun_apply_compose s fs t0) in UNI.
+        apply unfier_from_gt_unifier in UNI.
+        destruct UNI as [sc [SC_UNIFIES _]]. specialize (mgu_non_unifiable _ _ MGU sc).
+        contradiction. }
+      { red. exists (compose s d). exists n. split.
+        { constructor. }
+        { apply (denotational_sem_uni _ _ _ _ MGU); auto. } } }
+    { good_inversion OP. inversion EV; subst.
+      apply well_formedness_preservation in EV; auto. good_inversion EV. good_inversion wfState.
+      specialize (op_sem_exists (NTState (Leaf g1 s n))). intro p1. destruct p1 as [t1 OP1].
+      specialize (op_sem_exists (NTState (Leaf g2 s n))). intro p2. destruct p2 as [t2 OP2].
+      specialize (sum_op_sem _ _ _ _ _ OP1 OP2 OP0). intro Hinter.
+      good_inversion DSG.
+      { specialize (IHg1 f s n CG_G1 DSG0 DSS WF_L t1 OP1).
+        destruct IHg1 as [f' [HinDA ff'_eq]]. exists f'. split; auto.
+        red in HinDA. destruct HinDA as [sr [nr [Hin DSSr]]].
+        red. exists sr. exists nr. split; auto. constructor.
+        apply (interleave_in _ _ _ Hinter (Answer sr nr)). auto. }
+      { specialize (IHg2 f s n CG_G2 DSG0 DSS WF_R t2 OP2).
+        destruct IHg2 as [f' [HinDA ff'_eq]]. exists f'. split; auto.
+        red in HinDA. destruct HinDA as [sr [nr [Hin DSSr]]].
+        red. exists sr. exists nr. split; auto. constructor.
+        apply (interleave_in _ _ _ Hinter (Answer sr nr)). auto. } }
+    { good_inversion DSG. good_inversion OP. inversion EV; subst.
+      specialize (op_sem_exists (NTState (Leaf g1 s n))). intro p1. destruct p1 as [t1 OP1].
+      assert (wfst'1 : well_formed_nt_state (Leaf g1 s n)).
+      { constructor; good_inversion WF; auto. }
+      specialize (IHg1 f s n CG_G1 DSG_L DSS wfst'1 t1 OP1).
+      destruct IHg1 as [f' [HinDA ff'_eq]]. red in HinDA.
+      destruct HinDA as [s' [n' [Hinstr' HDAS']]].
+      specialize (op_sem_exists (NTState (Leaf g2 s' n'))). intro p2. destruct p2 as [t2 OP2].
+      specialize (counter_in_trace _ _ _ _ _ _ OP1 Hinstr'). intro n_le_n'.
+      assert (wfst'2 : well_formed_nt_state (Leaf g2 s' n')).
+      { good_inversion WF.
+        destruct (well_formed_subst_in_trace _ (wfNonTerminal _ wfst'1)  _ OP1 _ _ Hinstr').
+        intros. constructor; auto. intros.
+        apply lt_le_trans with n; auto. }
+      assert (Hg2' : in_denotational_sem_lev_goal (S l) g2 f').
+      { apply closedness_condition_lev with f; auto. intros. apply ff'_eq.
+        good_inversion WF. auto. }
+      specialize (IHg2 f' s' n' CG_G2 Hg2' HDAS' wfst'2 t2 OP2).
+      destruct IHg2 as [f'' [HinDA f'f''_eq]]. red in HinDA.
+      destruct HinDA as [s'' [n'' [Hinstr'' HDAS'']]].
+      exists f''. split.
+      { red. exists s''. exists n''. split; auto.
+        constructor. eapply prod_op_sem_in; eauto. }
+      { intros. red. apply eq_trans with (proj1_sig (f' x)).
+        { apply ff'_eq. auto. }
+        { apply f'f''_eq. omega. } } }
+    { good_inversion DSG. good_inversion OP. inversion EV; subst.
+      apply well_formedness_preservation in EV; auto. good_inversion EV.
+      rename fn into fa.
+      remember (fun x => if name_eq_dec x n
+                         then fa a
+                         else f x) as fn.
+      assert (Hgn : [| S l | g n , fn |]).
+      { good_inversion WF. apply den_sem_another_fresh_var with n a fa; auto.
+        { intro C. apply FV_LT_COUNTER in C. omega. }
+        {  destruct (name_eq_dec n n); try contradiction. reflexivity. }
+        { intros. destruct (name_eq_dec x n); try contradiction. auto. } }
+      assert (DSSn : [ s , fn ]).
+      { red. red in DSS. destruct DSS as [fs fssf'_eq].
+        remember (fun x => if name_eq_dec x n
+                         then fn n
+                         else fs x) as fs'.
+        exists fs'. red. intros. red. unfold subst_repr_fun_compose.
+        rewrite Heqfs'. rewrite Heqfn. destruct (name_eq_dec x n).
+        { assert (H_n_is_fresh_2 : apply_subst s (Var n) = Var n).
+          { simpl. destruct (image s n) eqn:eq; auto.
+            good_inversion WF. assert (n < n).
+            { apply DOM_LT_COUNTER. red. eauto. }
+            omega. }
+          rewrite e. rewrite H_n_is_fresh_2. simpl.
+          destruct (name_eq_dec n n); try contradiction. auto. }
+        { rewrite <- fssf'_eq. unfold subst_repr_fun_compose.
+          unfold apply_subst. destruct (image s x) eqn:eq.
+          { apply apply_repr_fun_fv. intros. good_inversion WF.
+            assert (in_subst_vran s x0). { red. eauto. }
+            destruct (name_eq_dec x0 n); try reflexivity.
+            apply VRAN_LT_COUNTER in H1. omega. }
+          { simpl. destruct (name_eq_dec x n); auto. omega. } } }
+      specialize (H n fn s (S n) (CG_BODY n) Hgn DSSn wfState t0 OP0).
+      destruct H as [f' [HinDA ff'_eq]]. exists f'. split.
+      { red. red in HinDA. destruct HinDA as [s' [n' [Hinstr HDAS]]].
+        exists s'. exists n'. split; auto. constructor; auto. }
+      { intros. assert (x < S n). { omega. }
+        specialize (ff'_eq x H0). red in ff'_eq. red. rewrite <- ff'_eq.
+        rewrite Heqfn. destruct (name_eq_dec x n); try omega. reflexivity. } }
+    { good_inversion DSG. good_inversion OP. inversion EV; subst.
+      apply well_formedness_preservation in EV; auto. good_inversion EV.
+      assert (cg_body : consistent_goal (proj1_sig (Language.Prog n) t)).
+      { remember (Language.Prog n) as d. destruct d as [rel [Hcl Hco]].
+        red in Hco. destruct (Hco t) as [Hcog Hcof]. auto. }
+      specialize (IHl (proj1_sig (Language.Prog n) t) f s n0 cg_body DSG0 DSS wfState t1 OP0).
+      destruct IHl as [f' [HinDA ff'_eq]]. exists f'. split; auto.
+      red. red in HinDA. destruct HinDA as [s' [n' [Hinstr HDAS]]].
+      exists s'. exists n'. split; auto. constructor; auto. } }
+Qed.
+
+Lemma search_completeness
+      (g   : goal)
+      (CG  : consistent_goal g)
+      (k   : nat)
+      (HC  : closed_goal_in_context (first_nats k) g)
+      (f   : repr_fun)
+      (t   : trace)
+      (OP : op_sem (NTState (Leaf g empty_subst k)) t)
+      (HDS : [| g , f |]) :
+      exists (f' : repr_fun), {| t , f' |} /\
+                            forall (x : name), In x (first_nats k) -> gt_eq (f x) (f' x).
+Proof.
+  apply in_denotational_sem_some_lev in HDS. destruct HDS as [l HDS].
+  assert (WF : well_formed_nt_state (Leaf g empty_subst k)).
+  { apply well_formed_initial_state; auto. }
+  specialize (search_completeness_generalized l g CG empty_subst k WF t OP f HDS (empty_subst_ds f)).
+  intro. destruct H as [f' [HinDA ff'eq]]. exists f'. split; auto.
+  intros. apply ff'eq. apply first_nats_less; auto.
+Qed.
