src/SLDSearch/OperationalSemSLD.v
@@ -1,0 +1,424 @@
+Require Import List.
+Import ListNotations.
+Require Import Coq.Lists.ListSet.
+Require Import Coq.Program.Equality.
+Require Import Omega.
+Require Import Extraction.
+
+Require Import Unification.
+Require Import Streams.
+Require Import LanguageSLD.
+Require Import DenotationalSemSLD.
+
+
+(************************* States *************************)
+
+Inductive cutting_mark : Set :=
+| StopCutting : cutting_mark
+| KeepCutting : cutting_mark.
+
+Inductive nt_state : Set :=
+| Leaf : goal -> subst -> nat -> nt_state
+| Sum  : cutting_mark -> nt_state -> nt_state -> nt_state
+| Prod : nt_state -> goal   -> nt_state.
+
+Inductive state : Set :=
+| Stop  : state
+| NTState : nt_state -> state.
+
+Inductive is_fv_of_nt_state : name -> nt_state -> Prop :=
+| isfvnstLeaf  : forall x g s n     (X_FV_G : is_fv_of_goal x g),
+                                    is_fv_of_nt_state x (Leaf g s n)
+| isfvnstSumL  : forall x m nst1 nst2 (X_FV : is_fv_of_nt_state x nst1),
+                                    is_fv_of_nt_state x (Sum m nst1 nst2)
+| isfvnstSumR  : forall x m nst1 nst2 (X_FV : is_fv_of_nt_state x nst2),
+                                    is_fv_of_nt_state x (Sum m nst1 nst2)
+| isfvnstProdL : forall x nst g     (X_FV : is_fv_of_nt_state x nst),
+                                    is_fv_of_nt_state x (Prod nst g)
+| isfvnstProdR : forall x nst g     (X_FV : is_fv_of_goal x g),
+                                    is_fv_of_nt_state x (Prod nst g).
+
+Hint Constructors is_fv_of_nt_state : core.
+
+Inductive is_fv_of_state : name -> state -> Prop :=
+| isfvstC : forall x nst (X_FV_NT_ST : is_fv_of_nt_state x nst),
+                         is_fv_of_state x (NTState nst).
+
+Hint Constructors is_fv_of_state : core.
+
+Inductive is_counter_of_nt_state : nat -> nt_state -> Prop :=
+| iscnstLeaf  : forall g s n,      is_counter_of_nt_state n (Leaf g s n)
+| iscnstSumL  : forall n m nst1 nst2 (ISC : is_counter_of_nt_state n nst1),
+                                   is_counter_of_nt_state n (Sum m nst1 nst2)
+| iscnstSumR  : forall n m nst1 nst2 (ISC : is_counter_of_nt_state n nst2),
+                                   is_counter_of_nt_state n (Sum m nst1 nst2)
+| iscnstProd  : forall n nst g     (ISC : is_counter_of_nt_state n nst),
+                                   is_counter_of_nt_state n (Prod nst g).
+
+Hint Constructors is_counter_of_nt_state : core.
+
+Inductive well_formed_nt_state : nt_state -> Prop :=
+| wfLeaf : forall g s frn
+           (DOM_LT_COUNTER  : forall x (X_IN_DOM : in_subst_dom s x), x < frn)
+           (VRAN_LT_COUNTER : forall x (X_IN_VRAN : in_subst_vran s x), x < frn)
+           (FV_LT_COUNTER   : forall x (X_FV : is_fv_of_goal x g), x < frn),
+           well_formed_nt_state (Leaf g s frn)
+| wfSum  : forall m nst1 nst2 (WF_L : well_formed_nt_state nst1)
+                            (WF_R : well_formed_nt_state nst2),
+                            well_formed_nt_state (Sum m nst1 nst2)
+| wfProd : forall nst g     (WF_L : well_formed_nt_state nst)
+                            (FV_LT_COUNTER : forall x frn (FRN_COUNTER : is_counter_of_nt_state frn nst)
+                                                          (X_FV : is_fv_of_goal x g),
+                                                          x < frn),
+                            well_formed_nt_state (Prod nst g).
+
+Hint Constructors well_formed_nt_state : core.
+
+Fixpoint first_nats (k : nat) : list nat :=
+  match k with
+  | 0   => []
+  | S n => n :: first_nats n
+  end.
+
+Lemma first_nats_less (n k : nat) (H : In n (first_nats k)) : n < k.
+Proof.
+  induction k.
+  { inversion H. }
+  { inversion H. { omega. } { apply IHk in H0. omega. } }
+Qed.
+
+Lemma well_formed_initial_state
+      (g   : goal)
+      (k   : nat)
+      (HC  : closed_goal_in_context (first_nats k) g) :
+      well_formed_nt_state (Leaf g empty_subst k).
+Proof.
+  constructor.
+  { intros. good_inversion X_IN_DOM. good_inversion H. }
+  { intros. good_inversion X_IN_VRAN. destruct H as [t0 [H0 _]]. good_inversion H0. }
+  { red in HC. intros. apply first_nats_less; auto. }
+Qed.
+
+
+Inductive well_formed_state : state -> Prop :=
+| wfTerminal    : well_formed_state Stop
+| wfNonTerminal : forall nst (wfState : well_formed_nt_state nst),
+                             well_formed_state (NTState nst).
+
+Hint Constructors well_formed_state : core.
+
+
+
+(************************** LTS ***************************)
+(* Labels *)
+Inductive label : Set :=
+| Step   : label
+| Answer : subst -> nat -> label.
+
+(* Cutting signal *)
+Inductive cut_signal : Set :=
+| NoCutting  : cut_signal
+| YesCutting : cut_signal.
+
+(* Transitions *)
+Inductive eval_step : nt_state -> label -> cut_signal -> state -> Prop :=
+| esFail         : forall s n, eval_step (Leaf Fail s n) Step NoCutting Stop
+| esCut          : forall s n, eval_step (Leaf Cut s n) (Answer s n) YesCutting Stop
+| esUnifyFail    : forall t1 t2 s   n (MGU : mgu (apply_subst s t1) (apply_subst s t2) None),
+                                      eval_step (Leaf (Unify t1 t2) s n) Step NoCutting Stop
+| esUnifySuccess : forall t1 t2 s d n (MGU : mgu (apply_subst s t1) (apply_subst s t2) (Some d)),
+                                      eval_step (Leaf (Unify t1 t2) s n) (Answer (compose s d) n) NoCutting Stop
+| esDisj         : forall g1 g2 s n, eval_step (Leaf (Disj g1 g2) s n)   Step NoCutting (NTState (Sum StopCutting (Leaf g1 s n) (Leaf g2 s n)))
+| esConj         : forall g1 g2 s n, eval_step (Leaf (Conj g1 g2) s n)   Step NoCutting (NTState (Prod (Leaf g1 s n) g2))
+| esFresh        : forall fg    s n, eval_step (Leaf (Fresh fg) s n)     Step NoCutting (NTState (Leaf (fg n) s (S n)))
+| esInvoke       : forall r arg s n, eval_step (Leaf (Invoke r arg) s n) Step NoCutting (NTState (Leaf (proj1_sig (LanguageSLD.Prog r) arg) s n))
+| esSumE         : forall m nst1       nst2 l (STEP_L : eval_step nst1 l NoCutting Stop),
+                                              eval_step (Sum m nst1 nst2) l NoCutting (NTState nst2)
+| esSumECS       : forall nst1         nst2 l (STEP_L : eval_step nst1 l YesCutting Stop),
+                                              eval_step (Sum StopCutting nst1 nst2) l NoCutting Stop
+| esSumECK       : forall nst1         nst2 l (STEP_L : eval_step nst1 l YesCutting Stop),
+                                              eval_step (Sum KeepCutting nst1 nst2) l YesCutting Stop
+| esSumNE        : forall m nst1 nst1' nst2 l (STEP_L : eval_step nst1 l NoCutting (NTState nst1')),
+                                              eval_step (Sum m nst1 nst2) l NoCutting (NTState (Sum m nst1' nst2))
+| esSumNECS      : forall nst1 nst1' nst2   l (STEP_L : eval_step nst1 l YesCutting (NTState nst1')),
+                                              eval_step (Sum StopCutting nst1 nst2) l NoCutting (NTState nst1')
+| esSumNECK      : forall nst1 nst1' nst2   l (STEP_L : eval_step nst1 l YesCutting (NTState nst1')),
+                                              eval_step (Sum KeepCutting nst1 nst2) l YesCutting (NTState nst1')
+| esProdSE       : forall nst g     cs      (STEP_L : eval_step nst Step cs Stop),
+                                            eval_step (Prod nst g) Step cs Stop
+| esProdAE       : forall nst g s n cs      (STEP_L : eval_step nst (Answer s n) cs Stop),
+                                            eval_step (Prod nst g) Step cs (NTState (Leaf g s n))
+| esProdSNE      : forall nst g     cs nst' (STEP_L : eval_step nst Step cs (NTState nst')),
+                                            eval_step (Prod nst g) Step cs (NTState (Prod nst' g))
+| esProdANE      : forall nst g s n cs nst' (STEP_L : eval_step nst (Answer s n) cs (NTState nst')),
+                                            eval_step (Prod nst g) Step cs (NTState (Sum KeepCutting (Leaf g s n) (Prod nst' g))).
+
+Hint Constructors eval_step : core.
+
+Lemma counter_in_answer
+      (nst : nt_state)
+      (s : subst)
+      (n : nat)
+      (cs : cut_signal)
+      (st : state)
+      (EV : eval_step nst (Answer s n) cs st) :
+      is_counter_of_nt_state n nst.
+Proof.
+  remember (Answer s n). induction EV; good_inversion Heql; auto.
+Qed.
+
+Lemma counter_in_next_state
+      (n : nat)
+      (nst nst_next : nt_state)
+      (l : label)
+      (cs : cut_signal)
+      (EV : eval_step nst l cs (NTState nst_next))
+      (ISC_NEXT :  is_counter_of_nt_state n nst_next) :
+      exists n', n' <= n /\ is_counter_of_nt_state n' nst.
+Proof.
+  remember (NTState nst_next) as st.
+  revert Heqst ISC_NEXT. revert nst_next.
+  induction EV; intros; good_inversion Heqst.
+  { exists n. split.
+    { constructor. }
+    { good_inversion ISC_NEXT; good_inversion ISC; auto. } }
+  { exists n. split.
+    { constructor. }
+    { good_inversion ISC_NEXT; good_inversion ISC; auto. } }
+  { good_inversion ISC_NEXT. exists n0. split.
+    { repeat constructor. }
+    { auto. } }
+  { exists n. split.
+    { constructor. }
+    { good_inversion ISC_NEXT; auto. } }
+  { exists n. split.
+    { constructor. }
+    { auto. } }
+  { specialize (IHEV nst1' eq_refl). good_inversion ISC_NEXT.
+    { apply IHEV in ISC. destruct ISC as [n' [LE ISC]].
+      exists n'; auto. } 
+    { exists n. split.
+      { constructor. }
+      { auto. } } }
+  { destruct (IHEV nst_next eq_refl ISC_NEXT) as [n' [LE ISC]].
+    exists n'; auto. }
+  { destruct (IHEV nst_next eq_refl ISC_NEXT) as [n' [LE ISC]].
+    exists n'; auto. }
+  { good_inversion ISC_NEXT. exists n0.
+    eapply counter_in_answer in EV. split; auto. }
+  { specialize (IHEV nst' eq_refl). good_inversion ISC_NEXT.
+    apply IHEV in ISC. destruct ISC as [n' [LE ISC]].
+    exists n'; auto. }
+  { specialize (IHEV nst' eq_refl). good_inversion ISC_NEXT.
+    { good_inversion ISC. exists n0.
+      eapply counter_in_answer in EV. split; auto. }
+    { good_inversion ISC. apply IHEV in ISC0.
+      destruct ISC0 as [n' [LE ISC]]. exists n'; auto. } }
+  
+Qed.
+
+Lemma well_formed_subst_in_answer
+      (nst : nt_state)
+      (s : subst)
+      (n : nat)
+      (cs : cut_signal)
+      (st : state)
+      (EV : eval_step nst (Answer s n) cs st)
+      (WF : well_formed_nt_state nst) :
+      (forall x, in_subst_dom s x -> x < n) /\ (forall x, in_subst_vran s x -> x < n).
+Proof.
+  remember (Answer s n). induction EV; good_inversion Heql; good_inversion WF; auto.
+  assert (FV_LT_N_1 : forall x, In x (fv_term (apply_subst s0 t1)) -> x < n).
+  { clear MGU. clear d. intros. induction t1.
+    { simpl in H. destruct (image s0 n0) eqn:eq; auto.
+      apply VRAN_LT_COUNTER. red. eauto. }
+    { good_inversion H. }
+    { simpl in H. apply (set_union_elim name_eq_dec) in H. destruct H.
+      { apply IHt1_1; auto. intros. apply FV_LT_COUNTER.
+        good_inversion X_FV; auto. apply fvUnifyL. simpl.
+        apply set_union_intro. left. auto. }
+      { apply IHt1_2; auto. intros. apply FV_LT_COUNTER.
+        good_inversion X_FV; auto. apply fvUnifyL. simpl.
+        apply set_union_intro. right. auto. } } }
+  assert (FV_LT_N_2 : forall x, In x (fv_term (apply_subst s0 t2)) -> x < n).
+  { clear MGU. clear d. intros. induction t2.
+    { simpl in H. destruct (image s0 n0) eqn:eq; auto.
+      apply VRAN_LT_COUNTER. red. eauto. }
+    { good_inversion H. }
+    { simpl in H. apply (set_union_elim name_eq_dec) in H. destruct H.
+      { apply IHt2_1; auto. intros. apply FV_LT_COUNTER.
+        good_inversion X_FV; auto. apply fvUnifyR. simpl.
+        apply set_union_intro. left. auto. }
+      { apply IHt2_2; auto. intros. apply FV_LT_COUNTER.
+        good_inversion X_FV; auto. apply fvUnifyR. simpl.
+        apply set_union_intro. right. auto. } } }
+  specialize (mgu_dom _ _ _ MGU). intro S'_DOM.
+  specialize (mgu_vran _ _ _ MGU). intro S'_VRAN.
+  split.
+  { intros. apply compose_dom in H. destruct H; auto.
+    apply S'_DOM in H. destruct H; auto. }
+  { intros. apply compose_vran in H. destruct H; auto.
+    apply S'_VRAN in H. destruct H; auto. }
+Qed.
+
+Lemma well_formedness_preservation
+      (nst : nt_state)
+      (l : label)
+      (cs : cut_signal)
+      (st : state)
+      (EV : eval_step nst l cs st)
+      (WF : well_formed_nt_state nst) :
+      well_formed_state st.
+Proof.
+  intros. induction EV; good_inversion WF; auto.
+  { constructor. auto. }
+  { constructor. constructor; auto.
+    intros. good_inversion FRN_COUNTER. subst. auto. }
+  { constructor. constructor; auto.
+    1-2: intros; eapply lt_trans; eauto.
+    intros. destruct (eq_nat_dec n x).
+    { omega. }
+    { apply Nat.lt_lt_succ_r. apply FV_LT_COUNTER. econstructor; eauto. } }
+  { constructor. constructor; auto.
+    specialize (proj2_sig (LanguageSLD.Prog r)). intro CC.
+    simpl in CC. destruct CC as [CL _]. red in CL. red in CL. auto. }
+  { specialize (IHEV WF_L).
+    good_inversion IHEV. auto. }
+  { constructor. constructor; auto.
+    1-2: apply well_formed_subst_in_answer in EV; destruct EV; auto.
+    intros. apply FV_LT_COUNTER; auto. eapply counter_in_answer; eauto. }
+  { specialize (IHEV WF_L). good_inversion IHEV.
+    constructor. constructor; auto. intros.
+    eapply counter_in_next_state in EV; eauto.
+    destruct EV as [frn' [LE ISC]]. eapply lt_le_trans.
+    2: eauto.
+    auto. }
+  { specialize (IHEV WF_L). good_inversion IHEV.
+    constructor. constructor.
+    { constructor.
+      1-2: apply well_formed_subst_in_answer in EV; destruct EV; auto.
+      intros. apply FV_LT_COUNTER; auto.
+      eapply counter_in_answer; eauto. }
+    { constructor; auto. intros.
+      eapply counter_in_next_state in EV; eauto.
+      destruct EV as [frn' [Le ISC]]. eapply lt_le_trans.
+      2: eauto.
+      auto. } }
+Qed.
+
+Lemma eval_step_exists
+      (nst : nt_state) :
+      {l : label & {cs : cut_signal & {st : state & eval_step nst l cs st}}}.
+Proof.
+  induction nst.
+  { destruct g.
+    1-2,4-7: repeat eexists; econstructor.
+    { assert ({r & mgu (apply_subst s t) (apply_subst s t0) r}).
+      { apply mgu_result_exists. }
+      destruct H. destruct x.
+      { repeat eexists; eauto. }
+      { repeat eexists; eauto. } } }
+  { destruct IHnst1 as [l1 [cs [st1 IH1]]].
+    destruct st1; destruct cs; destruct c.
+    all: repeat eexists; eauto. }
+  { destruct IHnst as [l [cs [st IH]]]. destruct st; destruct l.
+    all: repeat eexists; eauto. }
+Defined.
+
+Lemma eval_step_unique
+      (nst : nt_state)
+      (l1 l2 : label)
+      (cs1 cs2 : cut_signal)
+      (st1 st2 : state)
+      (STEP_1 : eval_step nst l1 cs1 st1)
+      (STEP_2 : eval_step nst l2 cs2 st2) :
+      l1 = l2 /\ cs1 = cs2 /\ st1 = st2.
+Proof.
+  revert STEP_1 STEP_2. revert l1 l2 cs1 cs2 st1 st2. induction nst.
+  { intros. destruct g; good_inversion STEP_1; good_inversion STEP_2; auto.
+    { assert (C : None = Some d).
+      { eapply mgu_result_unique; eassumption. }
+      inversion C. }
+    { assert (C : None = Some d).
+      { eapply mgu_result_unique; eassumption. }
+      inversion C. }
+    { assert (EQ : Some d = Some d0).
+      { eapply mgu_result_unique; eassumption. }
+      good_inversion EQ. auto. } }
+  { intros. good_inversion STEP_1; good_inversion STEP_2;
+    destruct (IHnst1 _ _ _ _ _ _ STEP_L STEP_L0) as [EQL [EQCS EQST]];
+    inversion EQCS; inversion EQST; subst; auto. }
+  { intros. good_inversion STEP_1; good_inversion STEP_2;
+    destruct (IHnst _ _ _ _ _ _ STEP_L STEP_L0)as [EQL [EQCS EQST]];
+    inversion EQL; inversion EQCS; inversion EQST; auto. }
+Qed.
+
+
+
+(***************** Operational Semantics ******************)
+
+Definition trace : Set := @stream label.
+
+CoInductive op_sem : state -> trace -> Prop :=
+| osStop : op_sem Stop Nil
+| osNTState : forall nst l cs st t (EV: eval_step nst l cs st)
+                                   (OP: op_sem st t),
+                                   op_sem (NTState nst) (Cons l t).
+
+Hint Constructors op_sem : core.
+
+CoFixpoint trace_from (st : state) : trace :=
+  match st with
+  | Stop => Nil
+  | NTState nst =>
+    match eval_step_exists nst with
+    | existT _ l (existT _ _ (existT _ nst' ev_nst_nst')) =>
+      Cons l (trace_from nst')
+    end
+  end.
+
+Lemma trace_from_correct
+      (st : state) :
+      op_sem st (trace_from st).
+Proof.
+  revert st. cofix CIH. destruct st.
+  { rewrite helper_eq. simpl. constructor. }
+  { rewrite helper_eq. simpl.
+    destruct (eval_step_exists n) as [l [cs [st EV]]].
+    econstructor; eauto. }
+Qed.
+
+Lemma op_sem_exists
+      (st : state) :
+      {t : trace & op_sem st t}.
+Proof.
+  eexists. eapply trace_from_correct.
+Defined.
+
+Lemma op_sem_unique
+      (st : state)
+      (t1 t2 : trace)
+      (OP_1 : op_sem st t1)
+      (OP_2 : op_sem st t2) :
+      equal_streams t1 t2.
+Proof.
+  revert OP_1 OP_2. revert t1 t2 st.
+  cofix CIH. intros. inversion OP_1; inversion OP_2;
+  rewrite <- H1 in H; inversion H.
+  { constructor. }
+  { subst.
+    destruct (eval_step_unique _ _ _ _ _ _ _ EV EV0) as [EQL [EQCS EQST]].
+    constructor.
+    { auto. }
+    { subst. eapply CIH; eauto. } }
+Qed.
+
+Definition in_denotational_analog (t : trace) (f : repr_fun) : Prop :=
+  exists (s : subst) (n : nat),
+    in_stream (Answer s n) t /\ [ s ,  f ].
+
+Notation "{| t , f |}" := (in_denotational_analog t f).
+
+Extraction Language Haskell.
+
+Extraction "extracted/sld_interpreter.hs" op_sem_exists.
