src/SLDSearch/SoundnessSLD.v
@@ -1,0 +1,123 @@
+Require Import List.
+Require Import Coq.Lists.ListSet.
+Import ListNotations.
+Require Import Omega.
+
+Require Import Unification.
+Require Import Streams.
+Require Import LanguageSLD.
+Require Import DenotationalSemSLD.
+Require Import OperationalSemSLD.
+
+Inductive in_denotational_sem_nt_state : nt_state -> repr_fun -> Prop :=
+| dsnstLeaf : forall g s n f (DSG  : [| g , f |])
+                             (DSS  : [ s , f ]),
+                             in_denotational_sem_nt_state (Leaf g s n) f
+| dsnstSumL : forall m nst1 nst2 f (DSST' : in_denotational_sem_nt_state nst1 f),
+                                 in_denotational_sem_nt_state (Sum m nst1 nst2) f
+| dsnstSumR : forall m nst1 nst2 f (DSST' : in_denotational_sem_nt_state nst2 f),
+                                 in_denotational_sem_nt_state (Sum m nst1 nst2) f
+| dsnstProd : forall nst g f (DSG : [| g , f |])
+                             (DSST' : in_denotational_sem_nt_state nst f),
+                             in_denotational_sem_nt_state (Prod nst g) f.
+
+Hint Constructors in_denotational_sem_nt_state : core.
+
+Inductive in_denotational_sem_state : state -> repr_fun -> Prop :=
+| dsstNTState : forall nst f (DSST' : in_denotational_sem_nt_state nst f),
+                           in_denotational_sem_state (NTState nst) f.
+
+Hint Constructors in_denotational_sem_state : core.
+
+
+Lemma answer_correct
+      (s : subst)
+      (n : nat)
+      (f : repr_fun)
+      (DSS : [ s , f ])
+      (st' : nt_state)
+      (cs : cut_signal)
+      (st : state)
+      (EV : eval_step st' (Answer s n) cs st) :
+      in_denotational_sem_nt_state st' f.
+Proof.
+  remember (Answer s n) as l.
+  induction EV; good_inversion Heql; auto.
+  { assert (DSS_copy := DSS). apply (denotational_sem_uni _ _ _ _ MGU _) in DSS.
+    destruct DSS as [DSS EQ]. constructor; auto. }
+Qed.
+
+Lemma next_state_correct
+      (f : repr_fun)
+      (st : state)
+      (DSS : in_denotational_sem_state st f)
+      (st' : nt_state)
+      (WF : well_formed_nt_state st')
+      (h : label)
+      (cs : cut_signal)
+      (EV : eval_step st' h cs st) :
+      in_denotational_sem_nt_state st' f.
+Proof.
+  induction EV; good_inversion DSS.
+  { good_inversion DSST'; good_inversion DSST'0;
+    constructor; auto. }
+  { good_inversion DSST'. good_inversion DSST'0. auto. }
+  { good_inversion WF. good_inversion DSST'.
+    constructor; auto. econstructor; eauto.
+    intros HIn. apply FV_LT_COUNTER in HIn.
+    { omega. }
+    { reflexivity. } }
+  { good_inversion DSST'. auto. }
+  { auto. }
+  { good_inversion WF. good_inversion DSST'; auto. }
+  { good_inversion WF. good_inversion DSST'; auto. }
+  { good_inversion WF. good_inversion DSST'; auto. }
+  { good_inversion DSST'. constructor; auto.
+    eapply answer_correct; eauto. }
+  { good_inversion WF. good_inversion DSST'. auto. }
+  { good_inversion WF. good_inversion DSST'.
+    { good_inversion DSST'0.
+      constructor; auto.
+      eapply answer_correct; eauto. }
+    { good_inversion DSST'0. auto. } }
+Qed.
+
+Lemma search_correctness_generalized
+      (st   : state)
+      (WF   : well_formed_state st)
+      (f    : repr_fun)
+      (t    : trace)
+      (HOP  : op_sem st t)
+      (HDA  : {| t , f |}) :
+      in_denotational_sem_state st f.
+Proof.
+  revert HOP WF. revert st.
+  red in HDA. destruct HDA as [s [n [HInStr DSS]]].
+  remember (Answer s n) as l. induction HInStr.
+  { intros. inversion HOP; clear HOP; subst.
+    constructor. eapply answer_correct; eauto. }
+  { specialize (IHHInStr Heql). intros.
+    inversion HOP; clear HOP; subst.
+    inversion WF; clear WF; subst.
+    specialize (well_formedness_preservation _ _ _ _ EV wfState).
+    intro wf_st0.
+    specialize (IHHInStr st0 OP wf_st0).
+    constructor. eapply next_state_correct; eauto. }
+Qed.
+
+Lemma search_correctness
+      (g   : goal)
+      (k   : nat)
+      (HC  : closed_goal_in_context (first_nats k) g)
+      (f   : repr_fun)
+      (t   : trace)
+      (HOP : op_sem (NTState (Leaf g empty_subst k)) t)
+      (HDA : {| t , f |}) :
+      [| g , f |].
+Proof.
+  remember (NTState (Leaf g empty_subst k)) as st.
+  assert (in_denotational_sem_state st f).
+  { eapply search_correctness_generalized; eauto.
+    subst. constructor. apply well_formed_initial_state; auto. }
+  subst. inversion H. inversion DSST'. auto.
+Qed.
