README.md
@@ -1,21 +1,27 @@
-# miniKanren-coq
 A certified semantics for relational programming workout.
 
-The folder 'src' contains the formalization of the system and all the proofs:
+`make` command will build and verify everything, and extract code from the Coq specification
 
-- Unify.v -- preliminaries from unification theory (terms, substitutions, computation of the most general unifier)
-- Stream.v -- (possibly infinite) streams and their properties 
-- MiniKanrenSyntax.v -- base language ('Prog' axiom here is an arbitrary correct program)
-- DenotationalSem.v -- denotational semantics
-- OperationalSem.v -- operational semantics for the interleaving search
-- OpSemSoundness.v -- soundness of the interleaving search
-- OpSemCompleteness.v -- completeness of the interleaving search
-- OperationalSemSLD.v -- operational semantics for the SLD search (with cuts)
-- OpSemSLDSoundness.v -- soundness of the SLD search (with cuts)
+The folder 'src' contains the specification of the semantics and all the proofs in Coq:
 
-The folder 'extracted' contains reference interpreters:
+- The subfolder 'src/Preliminaries' contains the specification of premilinary notions used in the semantics:
+    - Unification.v -- notions from unification theory (terms, substitutions, computation of the most general unifier)
+    - Streams.v -- (possibly infinite) streams and their properties 
+- The subfolder 'src/InterleavingSearch' contains the specification of syntax and semantics of miniKanren language with canonical interleaving search:
+    - Language.v -- base language ('Prog' axiom here is an arbitrary correct program)
+    - DenotationalSem.v -- denotational semantics
+    - OperationalSem.v -- operational semantics for interleaving search
+    - Soundness.v -- soundness of interleaving search
+    - Completeness.v -- completeness of interleaving search
+- The subfolder 'src/SLDSearch' contains the specification of syntax and semantics of miniKanren language with SLD resolution with cuts (it repeats the specification of interleaving search with minor modifications):
+    - LanguageSLD.v -- base language extended with ''cut'' constructs ('Prog' axiom here is an arbitrary correct program)
+    - DenotationalSemSLD.v -- denotational semantics
+    - OperationalSemSLD.v -- operational semantics for SLD resolution with cuts
+    - SoundnessSLD.v -- soundness of SLD resolution with cuts
 
-- interpreter.hs -- the code extracted from interleaving search semantics (from OperationalSem.v)
-- interpreter_wrapped.hs -- the code from interpreter_wrapped.hs appended with primitives for more convenient use and some tests
-- sld_interpreter.hs -- the code extracted from SLD search semantics (from OperationalSemSLD.v)
-- sld_interpreter_wrapped.hs -- the code from sld_interpreter_wrapped.hs appended with primitives for more convenient use (including the Prolog to MiniKanren translation) and some tests
+The folder 'extracted' contains reference interpreters extracted from the Coq specification:
+
+- interleaving_interpreter.hs -- the code extracted from interleaving search semantics (from src/InterleavingSearch/OperationalSem.v)
+- interleaving_interpreter_wrapped.hs -- the code from interleaving_interpreter.hs appended with primitives for more convenient use and some tests
+- sld_interpreter.hs -- the code extracted from SLD resolution with cuts semantics (from src/SLDSearch/OperationalSem.v)
+- sld_interpreter_wrapped.hs -- the code from sld_interpreter.hs appended with primitives for more convenient use (including the Prolog to MiniKanren translation) and some tests
